EvmYul/Yul/YulNotation.lean
@@ -309,7 +309,7 @@ partial def translateStmt (stmt : TSyntax `stmt) : TermElabM Term :=
   | `(stmt| $ids:ident,* := $expr:expr) => do
     let ids' := (ids : TSyntaxArray _).map translateIdent
     let expr ← translateExpr expr
-    `(Stmt.Let [$ids',*] (.some $expr))
+    `(Stmt.Assign [$ids',*] $expr)
 
   -- ExprStmt
   | `(stmt| $expr:expr) => do
@@ -373,10 +373,10 @@ example : <s break > = Stmt.Break := rfl
 example : <s let a, b := f(42) > = Stmt.Let ["a", "b"] (.some (.Call (Sum.inr "f") [Expr.Lit ⟨42⟩])) := rfl
 example : <s let a > = Stmt.Let ["a"] .none := rfl
 example : <s let a := 5 > = Stmt.Let ["a"] (.some (.Lit ⟨5⟩)) := rfl
-example : <s a, b := f(42) > = Stmt.Let ["a", "b"] (.some (.Call (Sum.inr "f") [Expr.Lit ⟨42⟩])) := rfl
-example : <s a := 42 > = Stmt.Let ["a"] (.some (.Lit ⟨42⟩)) := rfl
+example : <s a, b := f(42) > = Stmt.Assign ["a", "b"] (.Call (Sum.inr "f") [Expr.Lit ⟨42⟩]) := rfl
+example : <s a := 42 > = Stmt.Assign ["a"] (.Lit ⟨42⟩) := rfl
 
-example : <s c := add(a, b) > = Stmt.Let ["c"] (.some (Expr.Call (Sum.inl (Operation.StopArith Operation.SAOp.ADD)) [Expr.Var "a", Expr.Var "b"])) := rfl
+example : <s c := add(a, b) > = Stmt.Assign ["c"] (Expr.Call (Sum.inl (Operation.StopArith Operation.SAOp.ADD)) [Expr.Var "a", Expr.Var "b"]) := rfl
 example : <s let c := sub(a, b) > = Stmt.Let ["c"] (.some (Expr.Call (Sum.inl (Operation.StopArith Operation.SAOp.SUB)) [Expr.Var "a", Expr.Var "b"])) := rfl
 example : <s let a := 5 > = Stmt.Let ["a"] (.some (.Lit ⟨5⟩)) := rfl
 example : <s {} >
